rt spec+proof: prove decodeSchedContextInvocation_ccorres
This proves decodeSchedContextInvocation_ccorres, together with
many subsidiary results, including

- schedContext_unbindNtfn_ccorres
- schedContext_unbindTCB_ccorres
- schedContext_unbindAllTCBs_ccorres
- schedContext_updateConsumed_ccorres
- schedContext_completeYieldTo_ccorres
- decodeSchedContext_UnbindObject_ccorres
- decodeSchedContext_Bind_ccorres
- setConsumed_ccorres
- decodeSchedContext_YieldTo_ccorres

Substantial changes to the ASpec and the Haskell were made in order
to align with the C, as in seL4 PR#1435. In particular, the ASpec and
the Haskell use return_consumed and returnConsumed, respectively,
together with reply_from_kernel and replyFromKernel, in order to
respect the kernel reply protocol.

Signed-off-by: Michael McInerney <michael.mcinerney@proofcraft.systems>

spec/haskell/src/SEL4/Object/ObjectType.lhs
@@ -449,7 +449,7 @@ The "decodeInvocation" function parses the message, determines the operation tha
 >     liftM (uncurry InvokeDomain) $ decodeDomainInvocation label args extraCaps
 >
 > decodeInvocation label args _ _ (SchedContextCap {capSchedContextPtr=sc}) extraCaps False buffer =
->     liftM InvokeSchedContext $ decodeSchedContextInvocation label sc (map fst extraCaps) buffer
+>     liftM InvokeSchedContext $ decodeSchedContextInvocation label sc (map fst extraCaps)
 >
 > decodeInvocation label args _ _ SchedControlCap extraCaps False _ =
 >     liftM InvokeSchedControl $ decodeSchedControlInvocation label args (map fst extraCaps)
@@ -526,9 +526,8 @@ This function just dispatches invocations to the type-specific invocation functi
 >     withoutPreemption $ invokeIRQHandler invok
 >     return $ []
 >
-> performInvocation _ _ _ (InvokeSchedContext invok) = do
+> performInvocation _ _ _ (InvokeSchedContext invok) =
 >     withoutPreemption $ invokeSchedContext invok
->     return $ []
 >
 > performInvocation _ _ _ (InvokeSchedControl invok) = do
 >     withoutPreemption $ invokeSchedControlConfigureFlags invok
